compiler/correctness/miniMLExtraScript.sml
@@ -1,4 +1,4 @@
-open HolKernel bossLib boolLib boolSimps alistTheory listTheory rich_listTheory pred_setTheory lcsymtacs SatisfySimps
+open HolKernel bossLib boolLib boolSimps pairTheory alistTheory listTheory rich_listTheory pred_setTheory lcsymtacs SatisfySimps
 open MiniMLTheory MiniMLTerminationTheory miscTheory compileTerminationTheory
 val _ = new_theory "miniMLExtra"
 
@@ -570,5 +570,137 @@ val good_cenv_def = Define`
   ∀c n s. (MEM (c,(n,s)) cenv) ⇒
     c ∈ s ∧
     ∀c' n' s'. MEM (c',(n',s')) cenv ∧ c' ∈ s' ⇒ (s = s')`
+
+(* TODO: categorise *)
+
+val build_rec_env_MAP = store_thm("build_rec_env_MAP",
+  ``build_rec_env funs env = MAP (λ(f,x,e). (f, Recclosure env funs f)) funs ++ env``,
+  rw[build_rec_env_def] >>
+  qho_match_abbrev_tac `FOLDR (f env funs) env funs = MAP (g env funs) funs ++ env` >>
+  qsuff_tac `∀funs env env0 funs0. FOLDR (f env0 funs0) env funs = MAP (g env0 funs0) funs ++ env` >- rw[]  >>
+  unabbrev_all_tac >> simp[] >>
+  Induct >> rw[bind_def] >>
+  PairCases_on`h` >> rw[])
+
+val all_cns_def = tDefine "all_cns"`
+  (all_cns (Litv _) = {}) ∧
+  (all_cns (Conv cn vs) = cn INSERT BIGUNION (IMAGE all_cns (set vs))) ∧
+  (all_cns (Closure env _ _) = BIGUNION (IMAGE all_cns (set (MAP SND env)))) ∧
+  (all_cns (Recclosure env _ _) = BIGUNION (IMAGE all_cns (set (MAP SND env))))`
+  (WF_REL_TAC `measure v_size` >>
+   srw_tac[ARITH_ss][v1_size_thm,v3_size_thm] >>
+   Q.ISPEC_THEN`v_size`imp_res_tac SUM_MAP_MEM_bound >>
+   fsrw_tac[ARITH_ss][SUM_MAP_v2_size_thm])
+val all_cns_def = save_thm("all_cns_def",SIMP_RULE(srw_ss()++ETA_ss)[]all_cns_def)
+val _ = export_rewrites["all_cns_def"]
+
+val do_app_all_cns = store_thm("do_app_all_cns",
+  ``∀(cenv:envC) env op v1 v2 env' exp.
+      all_cns v1 ⊆ set (MAP FST cenv) ∧ all_cns v2 ⊆ set (MAP FST cenv) ∧
+      BIGUNION (IMAGE all_cns (set (MAP SND env))) ⊆ set (MAP FST cenv) ∧
+      (do_app env op v1 v2 = SOME (env',exp))
+      ⇒
+      BIGUNION (IMAGE all_cns (set (MAP SND env'))) ⊆ set (MAP FST cenv)``,
+  ntac 2 gen_tac >> Cases >>
+  Cases >> TRY (Cases_on`l`) >>
+  Cases >> TRY (Cases_on`l`) >>
+  rw[do_app_def] >> rw[] >>
+  fs[bind_def] >>
+  BasicProvers.EVERY_CASE_TAC >> rw[] >> rw[] >>
+  rw[build_rec_env_MAP,MAP_MAP_o,combinTheory.o_DEF,UNCURRY] >>
+  fsrw_tac[DNF_ss][SUBSET_DEF,MEM_MAP,FORALL_PROD,EXISTS_PROD] >>
+  metis_tac[])
+
+val pmatch_all_cns = store_thm("pmatch_all_cns",
+  ``(∀cenv p v env env'. (pmatch cenv p v env = Match env') ⇒
+    BIGUNION (IMAGE all_cns (set (MAP SND env'))) ⊆
+    all_cns v ∪ BIGUNION (IMAGE all_cns (set (MAP SND env)))) ∧
+    (∀cenv ps vs env env'. (pmatch_list cenv ps vs env = Match env') ⇒
+    BIGUNION (IMAGE all_cns (set (MAP SND env'))) ⊆
+    BIGUNION (IMAGE all_cns (set vs)) ∪
+    BIGUNION (IMAGE all_cns (set (MAP SND env))))``,
+  ho_match_mp_tac pmatch_ind >>
+  rw[pmatch_def,bind_def] >>
+  BasicProvers.EVERY_CASE_TAC >> fs[] >>
+  rfs[] >>
+  fsrw_tac[DNF_ss][SUBSET_DEF] >>
+  metis_tac[])
+
+val evaluate_all_cns = store_thm("evaluate_all_cns",
+  ``(∀cenv env exp res. evaluate cenv env exp res ⇒
+       (∀v. MEM v (MAP SND env) ⇒ all_cns v ⊆ set (MAP FST cenv)) ⇒
+       every_result (λv. all_cns v ⊆ set (MAP FST cenv)) res) ∧
+    (∀cenv env exps ress. evaluate_list cenv env exps ress ⇒
+       (∀v. MEM v (MAP SND env) ⇒ all_cns v ⊆ set (MAP FST cenv)) ⇒
+       every_result (EVERY (λv. all_cns v ⊆ set (MAP FST cenv))) ress) ∧
+    (∀cenv env v pes res. evaluate_match cenv env v pes res ⇒
+      (∀v. MEM v (MAP SND env) ⇒ all_cns v ⊆ set (MAP FST cenv)) ∧
+      all_cns v ⊆ set (MAP FST cenv) ⇒
+      every_result (λw. all_cns w ⊆ set (MAP FST cenv)) res)``,
+  ho_match_mp_tac evaluate_ind >>
+  strip_tac >- rw[] >>
+  strip_tac >- rw[] >>
+  strip_tac >- (
+    srw_tac[DNF_ss][MEM_MAP] >>
+    fs[do_con_check_def] >>
+    Cases_on `ALOOKUP cenv cn` >> fs[] >>
+    qexists_tac `(cn,x)` >>
+    imp_res_tac ALOOKUP_MEM >>
+    fs[] >>
+    fsrw_tac[DNF_ss][SUBSET_DEF,MEM_MAP,EVERY_MEM] >>
+    fsrw_tac[DNF_ss][MEM_EL,SUBSET_DEF] >>
+    metis_tac[EL_MAP] ) >>
+  strip_tac >- rw[] >>
+  strip_tac >- rw[] >>
+  strip_tac >- (
+    rw[] >>
+    imp_res_tac ALOOKUP_MEM >>
+    fsrw_tac[DNF_ss][MEM_MAP,FORALL_PROD] >>
+    metis_tac[] ) >>
+  strip_tac >- rw[] >>
+  strip_tac >- (
+    srw_tac[DNF_ss][SUBSET_DEF,MEM_MAP,FORALL_PROD,EXISTS_PROD] >>
+    metis_tac[] ) >>
+  strip_tac >- (
+    rw[] >> first_x_assum match_mp_tac >> fs[] >>
+    qspecl_then[`cenv`,`env`,`op`,`v1`,`v2`,`env'`,`exp''`]mp_tac do_app_all_cns >>
+    fsrw_tac[DNF_ss][SUBSET_DEF] >> metis_tac[]) >>
+  strip_tac >- rw[] >>
+  strip_tac >- rw[] >>
+  strip_tac >- rw[] >>
+  strip_tac >- rw[] >>
+  strip_tac >- rw[] >>
+  strip_tac >- rw[] >>
+  strip_tac >- rw[] >>
+  strip_tac >- rw[] >>
+  strip_tac >- rw[] >>
+  strip_tac >- rw[] >>
+  strip_tac >- rw[] >>
+  strip_tac >- (
+    rw[] >> fs[] >>
+    first_x_assum match_mp_tac >>
+    rw[bind_def] >> rw[]) >>
+  strip_tac >- rw[] >>
+  strip_tac >- (
+    rw[] >> fs[] >>
+    first_x_assum match_mp_tac >>
+    rw[build_rec_env_MAP,MAP_MAP_o,combinTheory.o_DEF,UNCURRY] >>
+    fsrw_tac[DNF_ss][MEM_MAP] >>
+    fsrw_tac[DNF_ss][SUBSET_DEF,MEM_MAP,FORALL_PROD,EXISTS_PROD] >>
+    metis_tac[]) >>
+  strip_tac >- rw[] >>
+  strip_tac >- rw[] >>
+  strip_tac >- rw[] >>
+  strip_tac >- rw[] >>
+  strip_tac >- rw[] >>
+  strip_tac >- rw[] >>
+  strip_tac >- (
+    rw[] >> first_x_assum match_mp_tac >>
+    imp_res_tac pmatch_all_cns >>
+    fsrw_tac[DNF_ss][SUBSET_DEF] >>
+    metis_tac[]) >>
+  strip_tac >- rw[] >>
+  strip_tac >- rw[] >>
+  strip_tac >- rw[])
 
 val _ = export_theory()
