compiler/correctness/bytecodeExtraScript.sml
@@ -1,5 +1,5 @@
-open HolKernel bossLib boolLib boolSimps lcsymtacs
-open bytecodeTerminationTheory
+open HolKernel bossLib boolLib boolSimps listTheory relationTheory arithmeticTheory lcsymtacs
+open miscTheory bytecodeTerminationTheory bytecodeEvalTheory
 val _ = intLib.deprecate_int()
 val _ = new_theory"bytecodeExtra"
 
@@ -37,5 +37,216 @@ val bc_find_loc_aux_MEM = store_thm("bc_find_loc_aux_MEM",
 
 val dest_Label_def = Define`(dest_Label (Label n) = n)`
 val _ = export_rewrites["dest_Label_def"]
+
+val is_Label_rwt = store_thm("is_Label_rwt",
+  ``∀i. is_Label i = ∃l. i = Label l``,
+  Cases >> rw[])
+
+val addr_of_el_def = Define`
+  (addr_of_el il n [] = NONE) ∧
+  (addr_of_el il n (x::xs) =
+   if n = 0 then if is_Label x then NONE else SOME 0 else
+     OPTION_BIND (addr_of_el il (n - 1) xs) (λm. SOME (m + (if is_Label x then 0 else il x + 1))))`
+val _ = export_rewrites["addr_of_el_def"]
+
+val bc_fetch_aux_addr_of_el = store_thm("bc_fetch_aux_addr_of_el",
+  ``∀c il pc n. (addr_of_el il n c = SOME pc) ⇒ (bc_fetch_aux c il pc = SOME (EL n c))``,
+  Induct >> rw[] >>
+  Cases_on `n` >> fs[] >>
+  spose_not_then strip_assume_tac >>
+  DECIDE_TAC)
+
+val bc_fetch_aux_not_label = store_thm("bc_fetch_aux_not_label",
+  ``∀c il pc i. (bc_fetch_aux c il pc = SOME i) ⇒ ¬is_Label i``,
+  Induct >> rw[] >> fs[] >> PROVE_TAC[])
+
+val labels_only_def = Define`
+  (labels_only (Jump (Addr _)) = F) ∧
+  (labels_only (JumpIf (Addr _)) = F) ∧
+  (labels_only (Call (Addr _)) = F) ∧
+  (labels_only (PushPtr (Addr _)) = F) ∧
+  (labels_only _ = T)`
+val _ = export_rewrites["labels_only_def"]
+
+val _ = Parse.overload_on("next_addr", ``λil ls. SUM (MAP (SUC o il) (FILTER ($~ o is_Label) ls))``)
+
+val bc_fetch_next_addr = store_thm("bc_fetch_next_addr",
+  ``∀bc0 bs x bc.
+    (bs.code = bc0 ++ (x::bc)) ∧ (¬is_Label x) ∧
+    (bs.pc = next_addr bs.inst_length bc0)
+    ⇒
+    (bc_fetch bs = SOME x)``,
+  Induct >- rw[bc_fetch_def] >>
+  rw[bc_fetch_def] >>
+  fsrw_tac[ARITH_ss][bc_fetch_def,ADD1] >>
+  first_x_assum (qspec_then `bs with <| code := TL bs.code ; pc := next_addr bs.inst_length bc0 |>` mp_tac) >>
+  rw[])
+
+val bc_find_loc_aux_thm = store_thm("bc_find_loc_aux_thm",
+  ``∀il ls l n.
+     bc_find_loc_aux ls il l n =
+     if MEM (Label l) ls then
+     SOME (n + SUM (MAP (SUC o il) (FILTER ($~ o is_Label) (TAKE (LEAST m. m < LENGTH ls ∧ (EL m ls = Label l)) ls))))
+     else NONE``,
+  gen_tac >> Induct >- rw[bc_find_loc_aux_def] >>
+  simp[bc_find_loc_aux_def] >>
+  qx_gen_tac `h` >> qx_gen_tac `l` >>
+  Cases_on `h = Label l` >> fs[] >- (
+    qx_gen_tac `n` >>
+    qmatch_abbrev_tac `n = n + m` >>
+    qsuff_tac `m = 0` >- rw[] >>
+    unabbrev_all_tac >>
+    numLib.LEAST_ELIM_TAC >>
+    conj_tac >- (
+      qexists_tac `0` >> rw[] ) >>
+    gen_tac >>
+    strip_tac >>
+    first_x_assum (qspec_then `0` mp_tac) >>
+    srw_tac[ARITH_ss][] ) >>
+  Cases_on `MEM (Label l) ls` >> fs[] >>
+  Q.PAT_ABBREV_TAC`l0 = $LEAST X` >>
+  Q.PAT_ABBREV_TAC`l1 = $LEAST X` >>
+  `(SUC l0) = l1` by (
+    unabbrev_all_tac >>
+    qmatch_abbrev_tac `SUC ($LEAST P) = X` >>
+    `∃n. P n` by (
+      fs[MEM_EL,Abbr`P`] >>
+      PROVE_TAC[] ) >>
+    rw[UNDISCH(Q.SPEC`n`SUC_LEAST)] >>
+    unabbrev_all_tac >>
+    AP_TERM_TAC >>
+    rw[FUN_EQ_THM] >>
+    Cases_on `m` >> rw[] ) >>
+  srw_tac[ARITH_ss][])
+
+val bc_find_loc_aux_ALL_DISTINCT = store_thm("bc_find_loc_aux_ALL_DISTINCT",
+  ``∀ls il l n z k. ALL_DISTINCT (FILTER is_Label ls) ∧ (k < LENGTH ls) ∧ (EL k ls = Label l) ∧
+    (z = n + next_addr il (TAKE k ls)) ⇒
+    (bc_find_loc_aux ls il l n = SOME z)``,
+  rw[bc_find_loc_aux_thm] >- (
+   rw[MEM_EL] >> PROVE_TAC[] ) >>
+  numLib.LEAST_ELIM_TAC >>
+  conj_tac >- PROVE_TAC[] >>
+  qx_gen_tac `j` >> rw[] >>
+  qsuff_tac `k = j` >> rw[] >>
+  match_mp_tac (Q.ISPEC`is_Label`ALL_DISTINCT_FILTER_EL_IMP) >>
+  qexists_tac `ls` >> rw[])
+
+val bc_fetch_aux_append_code = store_thm("bc_fetch_aux_append_code",
+  ``∀il ls n l2 i. (bc_fetch_aux ls il n = SOME i) ⇒ (bc_fetch_aux (ls ++ l2) il n = SOME i)``,
+    gen_tac >> Induct >> rw[bc_fetch_aux_def] )
+
+val bc_fetch_append_code = store_thm("bc_fetch_append_code",
+  ``(bc_fetch bs = SOME i) ⇒ (bc_fetch (bs with code := bs.code ++ c) = SOME i)``,
+  rw[bc_fetch_def] >>
+  imp_res_tac bc_fetch_aux_append_code >>
+  rw[] )
+
+val bc_find_loc_aux_append_code = store_thm("bc_find_loc_aux_append_code",
+  ``∀il ls n l2 l i. (bc_find_loc_aux ls il n l = SOME i) ⇒ (bc_find_loc_aux (ls ++ l2) il n l = SOME i)``,
+  gen_tac >> Induct >> rw[bc_find_loc_aux_def] )
+
+val bc_find_loc_append_code = store_thm("bc_find_loc_append_code",
+  ``(bc_find_loc bs l = SOME n) ⇒ (bc_find_loc (bs with code := bs.code ++ c) l = SOME n)``,
+  Cases_on `l` >> rw[bc_find_loc_def] >>
+  imp_res_tac bc_find_loc_aux_append_code >>
+  rw[] )
+
+val bc_state_component_equality = save_thm("bc_state_component_equality",
+DB.fetch"Bytecode""bc_state_component_equality")
+
+val bc_next_append_code = store_thm("bc_next_append_code",
+  ``∀bs1 bs2. bc_next bs1 bs2 ⇒ ∀c0 c. (bs1.code = c0) ⇒ bc_next (bs1 with code := c0 ++ c) (bs2 with code := c0 ++ c)``,
+  ho_match_mp_tac bc_next_ind >>
+  strip_tac >- (
+    rw[bc_eval1_thm] >>
+    imp_res_tac bc_fetch_append_code >>
+    rw[bc_eval1_def] >>
+    fs[bc_eval_stack_thm] >>
+    rw[bump_pc_def] ) >>
+  strip_tac >- (
+    rw[bc_eval1_thm] >>
+    imp_res_tac bc_fetch_append_code >>
+    imp_res_tac bc_find_loc_append_code >>
+    rw[bc_eval1_def] ) >>
+  strip_tac >- (
+    rw[bc_eval1_thm] >>
+    imp_res_tac bc_fetch_append_code >>
+    imp_res_tac bc_find_loc_append_code >>
+    rw[bc_eval1_def,LET_THM] >>
+    rw[bump_pc_with_stack] >>
+    rw[bump_pc_def] ) >>
+  strip_tac >- (
+    rw[bc_eval1_thm] >>
+    imp_res_tac bc_fetch_append_code >>
+    imp_res_tac bc_find_loc_append_code >>
+    rw[bc_eval1_def,LET_THM] >>
+    rw[bc_state_component_equality] >>
+    rw[bump_pc_def] ) >>
+  strip_tac >- (
+    rw[bc_eval1_thm] >>
+    imp_res_tac bc_fetch_append_code >>
+    imp_res_tac bc_find_loc_append_code >>
+    rw[bc_eval1_def,LET_THM] >>
+    rw[bc_state_component_equality] >>
+    rw[bump_pc_def] ) >>
+  strip_tac >- (
+    rw[bc_eval1_thm] >>
+    imp_res_tac bc_fetch_append_code >>
+    rw[bc_eval1_def,LET_THM] ) >>
+  strip_tac >- (
+    rw[bc_eval1_thm] >>
+    imp_res_tac bc_fetch_append_code >>
+    imp_res_tac bc_find_loc_append_code >>
+    rw[bc_eval1_def,LET_THM] >>
+    rw[bc_state_component_equality] >>
+    rw[bump_pc_def] ) >>
+  strip_tac >- (
+    rw[bc_eval1_thm] >>
+    imp_res_tac bc_fetch_append_code >>
+    imp_res_tac bc_find_loc_append_code >>
+    rw[bc_eval1_def,LET_THM] ) >>
+  strip_tac >- (
+    rw[bc_eval1_thm] >>
+    imp_res_tac bc_fetch_append_code >>
+    imp_res_tac bc_find_loc_append_code >>
+    rw[bc_eval1_def,LET_THM] ) >>
+  strip_tac >- (
+    rw[bc_eval1_thm] >>
+    imp_res_tac bc_fetch_append_code >>
+    imp_res_tac bc_find_loc_append_code >>
+    rw[bc_eval1_def,LET_THM] >>
+    rw[bump_pc_def]) >>
+  strip_tac >- (
+    rw[bc_eval1_thm] >>
+    imp_res_tac bc_fetch_append_code >>
+    imp_res_tac bc_find_loc_append_code >>
+    rw[bc_eval1_def,LET_THM] >>
+    rw[bump_pc_def]) >>
+  rw[bc_eval1_thm] >>
+  imp_res_tac bc_fetch_append_code >>
+  imp_res_tac bc_find_loc_append_code >>
+  rw[bc_eval1_def,LET_THM] >>
+  rw[bump_pc_def])
+
+val bc_next_preserves_code = store_thm("bc_next_preserves_code",
+  ``∀bs1 bs2. bc_next bs1 bs2 ⇒ (bs2.code = bs1.code)``,
+  ho_match_mp_tac bc_next_ind >>
+  rw[bump_pc_def] >>
+  BasicProvers.EVERY_CASE_TAC >> rw[])
+
+val RTC_bc_next_append_code = store_thm("RTC_bc_next_append_code",
+  ``∀bs1 bs2 bs1c bs2c c. RTC bc_next bs1 bs2 ∧
+    (bs1c = bs1 with code := bs1.code ++ c) ∧
+    (bs2c = bs2 with code := bs2.code ++ c)
+    ⇒ RTC bc_next bs1c bs2c``,
+  rw[] >> (
+     RTC_lifts_monotonicities
+  |> Q.GEN`R` |> Q.ISPEC `bc_next`
+  |> Q.GEN`f` |> Q.SPEC `λbs. bs with code := bs.code ++ c`
+  |> strip_assume_tac) >> fs[] >> pop_assum (match_mp_tac o MP_CANON) >>
+  rw[] >>
+  imp_res_tac bc_next_append_code >> fs[] >>
+  metis_tac[bc_next_preserves_code])
 
 val _ = export_theory()
